\section{Simulations}

\subsection{Simple case}

\begin{equation*}
    G(z^{-1}) = \frac{0.25 z^{-1}}{1 - 0.75 z^{-1}}
\end{equation*}

\begin{equation*}
    K(z^{-1}) = 0.6 + 0.3 \frac{z^{-1}}{1-z^{-1}} = \frac{0.6 - 0.3z^{-1}}{1-z^{-1}} = 
    \begin{bmatrix}
        \frac{1}{1-z^{-1}} & \frac{z^{-1}}{1-z^{-1}}
    \end{bmatrix} 
    \begin{bmatrix}
        0.6 \\ -0.3
    \end{bmatrix}
\end{equation*}

\begin{equation*}
    M(z^{-1}) = \frac{K(z^{-1}) G(z^{-1})}{1+K(z^{-1})G(z^{-1})} = \frac{0.15 z^{-1} - 0.075 z^{-2}}{1 - 1.6 z^{-1} + 0.675 z^{-2}}
\end{equation*}


\todo[inline]{Bla bla bla, see figure \ref{fig:simple_case_transient_removed}.}

\begin{figure}
    \centering
    \includegraphics[width =\textwidth]{figures/Transient_removed_noiseless_no_constr.eps}
    \caption{Resulting closed loop systems, with and without transient removal. $l_1 = 63$ (all correlation lags). Transient removed with the robust polynomial method for periodic signals (order = 2).}
    \label{fig:simple_case_transient_removed}
\end{figure}